Improve iforest definition + first useful lemmas

utils/iforestScript.sml
@@ -3,107 +3,304 @@ open llistTheory optionTheory itreesTheory finite_mapTheory;
 
 val _ = new_theory "iforest";
 
-(* Type aliases *)
+(* iforest abstract definition *)
+
+Datatype:
+  itree_action = Ext 'a | Int | Res 'r
+End
 
 (* An Itree with a action ('a), event ('e), and result ('r) types *)
 val itree  = “itree  : ('a,'e,'r) itree”
+val itree' = “itree' : ('a,'e,'r) itree”
 
 (* A forest is a finite mapping from some kind of identifier to an Itree *)
-val forest = “forest : 'p |-> ('a,'e,'r) itree”
+val _       = type_abbrev("forest",“:'p |-> ('a,'e,'r) itree”)
+val forest  = “forest   : ('r,'e,'a,'p) forest”
+val forest' = “forest'  : ('r,'e,'a,'p) forest”
 
 (* Given an Itree identifier and an event which action should we perform? *)
-val act    = “act    : 'p -> 'e -> 'a option”
+val _    = type_abbrev("act",“:'p -> 'e -> 'a option”)
+val act  = “act  : ('a,'e,'p) act”
+val act' = “act' : ('a,'e,'p) act”
 
 (* Given an (act)ed on Itree and event, how shoudl we update act? *)
-val upd    = “upd    : 'p -> 'e ->
-                       ('p -> 'e -> 'a option) ->
-                       'p -> 'e -> 'a option”
+val _    = type_abbrev("upd",“:'p -> 'e -> ('a,'e,'p) act -> ('a,'e,'p) act”)
+val upd  = “upd  : ('a,'e,'p) upd”
+val upd' = “upd' : ('a,'e,'p) upd”
 
+Datatype:
+  iforest = <| forest : 'p |-> ('a,'e,'r) itree ;
+               act    : 'p -> 'e -> 'a option;
+               upd    : 'p -> 'e ->
+                        ('p -> 'e -> 'a option) ->
+                         'p -> 'e -> 'a option
+|>
+End
+
+val iforest = “ψ  :('a,'e,'p,'r) iforest”
+val psi     = “ψ  :('a,'e,'p,'r) iforest”
+val psi'    = “ψ' :('a,'e,'p,'r) iforest”
+
+
+(* iforest basic operations *)
+
+Definition iforest_get_def:
+  iforest_get ^iforest p = FLOOKUP ψ.forest p
+End
+
+Definition iforest_set_def:
+  iforest_set ^iforest p i = ψ with forest := ψ.forest |+ (p,i)
+End
+
+Definition iforest_del_def:
+  iforest_del ^iforest p = ψ with forest := ψ.forest \\ p
+End
+
+Definition iforest_upd_act_def:
+  iforest_upd_act ^iforest p e = ψ with act := ψ.upd p e ψ.act
+End
+
+Definition iforest_upd_def:
+  iforest_upd ^iforest p e f =
+    case ψ.act p e of
+      NONE   => ψ
+    | SOME a => ψ with <| forest := ψ.forest |+ (p,f a); act := ψ.upd p e ψ.act |>
+End
+
+Theorem iforest_upd_alt_def:
+∀ψ p e f.
+  IS_SOME (ψ.act p e) ⇒
+  iforest_upd ψ p e f = iforest_upd_act (iforest_set ψ p (f (THE (ψ.act p e)))) p e
+Proof
+  rw[iforest_upd_def,iforest_set_def,iforest_upd_act_def,IS_SOME_EXISTS]
+  \\ simp[]
+QED
+
+Definition iforest_itrees_def:
+  iforest_itrees ^iforest = FDOM ψ.forest
+End
+
+Definition iforest_can_act_def:
+  iforest_can_act ^iforest p =
+  case iforest_get ψ p of
+    NONE => F
+  | SOME (Vis e f) => IS_SOME (ψ.act p e)
+  | _ => T
+End
 
 (* A trace is a stream of Itree identifiers to operate over.
    It is meant to represent in which order the forest is being
    evaluated. For most useful proofs about a forest some notion
    of fair trace might be needed.
 *)
-val trace  = “trace  : 'p llist”
+val trace   = “trace   : 'p llist”
+val trace'  = “trace'  : 'p llist”
+
+Definition next_proc_def:
+  next_proc ^iforest trace =
+    case LFILTER (λp. p ∈ iforest_itrees ψ ∧ iforest_can_act ψ p) trace of
+      [||] => NONE
+    | p:::ll => SOME (p,ll)
+End
+
+(* Properties of the basic iforest operations *)
+
+Theorem next_proc_ifores_get_SOME:
+  ∀ψ trace p ll.
+    next_proc ψ trace = SOME (p,ll)
+    ⇒ ∃i. iforest_get ψ p = SOME i
+Proof
+  rw[next_proc_def]
+  \\ gs[CaseEq"llist"]
+  \\ drule LFILTER_EQ_CONS
+  \\ rw[iforest_can_act_def]
+  \\ Cases_on ‘iforest_get ψ p’
+  \\ gs[]
+QED
+
+Theorem iforest_itrees_del:
+  ∀ψ p.
+    p ∉ iforest_itrees (iforest_del ψ p)
+Proof
+  simp[iforest_del_def,iforest_itrees_def]
+QED
+
+Definition iforest_step_def:
+  (* If the Itree is done, remove it from the forest *)
+  iforest_step ψ p (Ret t)   = iforest_del ψ p
+  (* If the Itree is in an internal transition simply update it *)
+∧ iforest_step ψ p (Tau t)   = iforest_set ψ p t
+  (* If the Itree returns an event:  *)
+  (* We must likely can act on it (from next_proc)  *)
+  (* So, we update the act function according to upd
+        and record the event to the stream. *)
+∧ iforest_step ψ p (Vis e f) = iforest_upd ψ p e f
+End
+
+Definition iforest_act_def:
+  iforest_act ψ p (Ret t)   = (p,Res t)
+∧ iforest_act ψ p (Tau t)   = (p,Int)
+∧ iforest_act ψ p (Vis e f) = (p,Ext e)
+End
+
+Theorem iforest_act_FST:
+  ∀ψ p i. FST (iforest_act ψ p i) = p
+Proof
+  Cases_on ‘i’ \\ gs[iforest_act_def]
+QED
 
 (* Folding function to be used with  LUNFOLD *)
 Definition iforest_aux1_def:
-  (* If the stream is empty we are done *)
-  iforest_aux (^act,^upd,^forest,[||]) = NONE
-  (* When an Itree p is selected *)
-∧ iforest_aux (^act,^upd,^forest,p:::^trace) =
-  (* Check if the Itree is in the forest *)
-  case FLOOKUP forest p of
-    (* If there is no such ITree, move on, this is (somewhat) weird *)
-    NONE           => SOME ((act,upd,forest,trace),NONE)
-  (* If the Itree has return, move on to another Itree (continue) *)
-  | SOME (Ret t)   => SOME ((act,upd,forest,trace),NONE)
-  (* If the Itree is in an internal transition advance and update the Iforest *)
-  | SOME (Tau t)   => SOME ((act,upd,forest |+ (p, t),trace),NONE)
-  (* If the Itree returns an event:  *)
-  | SOME (Vis e f) =>
-      (* See if we can act on it *)
-      case act p e of
-        (* If we (currently) can not act, then move on to anaother Itree.
-           The hope here is that maybe after some other Itrees in the forest
-           have been acted on we could come back and be able to do something.
-         *)
-        NONE   => SOME ((act,upd,forest,trace),NONE)
-      (* If we can act, do so and update the act function according to upd.
-         Once we act on an event we record it to the stream
-       *)
-      | SOME a => SOME ((upd p e act,upd,forest |+ (p, f a),trace),SOME e)
+  iforest_aux (^iforest,^trace) =
+  case next_proc ψ trace of
+    NONE => NONE
+  | SOME (p,ll) =>
+      case iforest_get ψ p of
+        NONE   => NONE
+      | SOME i => SOME ((iforest_step ψ p i,ll),iforest_act ψ p i)
 End
 
 (* To create the stream of events we filter out all the NONE element from
    Ret and Tau Itrees
 *)
 Definition iforest_aux_def:
-  iforest ^act ^upd ^forest ^trace =
-    LMAP THE (LFILTER IS_SOME (LUNFOLD iforest_aux (act,upd,forest,trace)))
+  iforest ^iforest ^trace =
+    LUNFOLD iforest_aux (ψ,trace)
 End
 
 (* Much nicer version of iforest.
    - Comments are duplicated from iforest_aux1_def
  *)
-
 Theorem iforest_def[compute]:
-∀ ^act ^upd ^forest p ^trace.
-  (* If the stream is empty we are done *)
-  iforest act upd forest  [||] = [||]
-  (* When an Itree p is selected *)
-∧ iforest act upd forest (p:::^trace) =
-  (* Check if the Itree is in the forest *)
-  case FLOOKUP forest p of
-    (* If there is no such ITree, move on, this is (somewhat) weird *)
-    NONE           => iforest act upd forest             trace
-  (* If the Itree has return, move on to another Itree (continue) *)
-  | SOME (Ret t)   => iforest act upd forest             trace
-  (* If the Itree is in an internal transition advance and update the Iforest *)
-  | SOME (Tau t)   => iforest act upd (forest |+ (p, t)) trace
-  (* If the Itree returns an event:  *)
-  | SOME (Vis e f) =>
-      (* See if we can act on it *)
-      case act p e of
-        (* If we (currently) can not act, then move on to anaother Itree.
-           The hope here is that maybe after some other Itrees in the forest
-           have been acted on we could come back and be able to do something.
-         *)
-        NONE   => iforest act upd forest trace
-      (* If we can act, do so and update the act function according to upd.
-         Once we act on an event we record it to the stream
-       *)
-      | SOME a => e ::: iforest (upd p e act) upd (forest |+ (p, f a)) trace
+∀ ^iforest ^trace.
+  iforest ^iforest ^trace =
+  case next_proc ψ trace of
+    NONE => [||]
+  | SOME (p,ll) =>
+      let i = THE (iforest_get ψ p)
+      in iforest_act ψ p i ::: iforest (iforest_step ψ p i) ll
 Proof
-  rw[iforest_aux_def]
-  >- simp[Once LUNFOLD,iforest_aux1_def]
-  \\ Cases_on ‘FLOOKUP forest p’
-  >- simp[Once LUNFOLD,iforest_aux1_def]
-  \\ Cases_on ‘x’
-  >~ [‘Vis a g’]
-  >- (Cases_on ‘act p a’ \\ simp[Once LUNFOLD,iforest_aux1_def])
-  \\ simp[Once LUNFOLD,iforest_aux1_def]
+  rw[iforest_aux_def,Once iforest_aux1_def,Once LUNFOLD]
+  \\ Cases_on ‘next_proc ψ trace’ \\ gs[]
+  \\ Cases_on ‘x’ \\ gs[]
+  \\ drule next_proc_ifores_get_SOME \\ rw[]
+  \\ simp[]
+QED
+
+Theorem iforest_alt_def:
+∀ ^iforest ^trace.
+  iforest ^iforest ^trace =
+  case next_proc ψ trace of
+    NONE => [||]
+  | SOME (p,ll) =>
+      case iforest_get ψ p of
+        NONE => [||]
+      | SOME i => iforest_act ψ p i ::: iforest (iforest_step ψ p i) ll
+Proof
+  rw[iforest_aux_def,Once iforest_aux1_def,Once LUNFOLD]
+  \\ Cases_on ‘next_proc ψ trace’ \\ gs[]
+  \\ Cases_on ‘x’ \\ gs[]
+  \\ drule next_proc_ifores_get_SOME \\ rw[]
+  \\ simp[]
+QED
+
+Theorem iforest_eq:
+  ∀R ^iforest ^trace res.
+    R ψ trace res ∧
+    (∀^iforest ^trace res.
+      R ψ trace res ⇒
+        (IS_NONE (next_proc ψ trace) ∧ res = [||]) ∨
+        (∃p ll i res'.
+           next_proc ψ trace = SOME (p,ll) ∧
+           iforest_get ψ p = SOME i ∧
+           res = iforest_act ψ p i:::res' ∧
+           R (iforest_step ψ p i) ll res')) ⇒
+    (iforest ψ trace = res)
+Proof
+  rw[]
+  \\ rw[Once LLIST_BISIMULATION]
+  \\ qexists_tac
+     ‘λll1 ll2.
+        ∃^iforest trace.
+          ll1 = iforest ψ trace ∧ R ψ trace ll2’
+  \\ rw[]
+  >- metis_tac []
+  \\ res_tac \\ rw[]
+  \\ gs[Once iforest_def]
+  \\ metis_tac []
+QED
+
+Theorem iforest_itrees_mono_step:
+  ∀i ψ p. p ∈ iforest_itrees ψ ⇒ iforest_itrees (iforest_step ψ p i) ⊆ iforest_itrees ψ
+Proof
+  rw[] \\ Cases_on ‘i’ \\ EVAL_TAC
+  \\ gs[FDOM_DRESTRICT,iforest_itrees_def]
+  \\ Cases_on ‘ψ.act p a’ \\ gs[]
+QED
+
+Theorem not_in_forest_not_in_trace:
+  ∀p ^psi trace.
+    p ∉ iforest_itrees ψ
+    ⇒ every (λ(q,a). p ≠ q) (iforest ψ trace)
+Proof
+  rw[]
+  \\ ho_match_mp_tac (MP_CANON every_strong_coind)
+  \\ qexists_tac ‘λll. ∃^psi' trace. ll = iforest ψ' trace ∧  iforest_itrees ψ' ⊆ iforest_itrees ψ’
+  \\ rw[]
+  >- (Cases_on ‘h’ \\ rw[] \\ gs[Once iforest_def]
+      \\ Cases_on ‘next_proc ψ' trace’ \\ gs[]
+      \\ Cases_on ‘x’ \\ gs[] \\ rveq
+      \\ first_x_assum (assume_tac o Q.AP_TERM ‘FST’)
+      \\ gs[iforest_act_FST] \\ rveq
+      \\ ‘p ∉ iforest_itrees ψ'’
+         by (gs[SUBSET_DEF] \\ CCONTR_TAC \\ gs[])
+      \\ gs[next_proc_def,CaseEq"llist"]
+      \\ drule LFILTER_EQ_CONS
+      \\ rw[] \\ CCONTR_TAC \\ gs[])
+  >- (Cases_on ‘h’ \\ rw[] \\ gs[Once iforest_def]
+      \\ Cases_on ‘next_proc ψ' trace’ \\ gs[]
+      \\ Cases_on ‘x’ \\ gs[] \\ rveq
+      \\ disj1_tac \\ qexists_tac ‘iforest_step ψ' q' (THE (iforest_get ψ' q'))’
+      \\ qexists_tac ‘r'’ \\ simp[]
+      \\ irule SUBSET_TRANS \\ first_x_assum (irule_at Any) \\ simp[]
+      \\ irule iforest_itrees_mono_step
+      \\ gs[next_proc_def,CaseEq"llist"]
+      \\ drule LFILTER_EQ_CONS
+      \\ rw[])
+  >- (qexists_tac ‘ψ’ \\ simp[] \\ metis_tac [])
+QED
+
+Theorem iforest_not_in_forest:
+  ∀n ^iforest trace p a.
+    p ∉ iforest_itrees ψ
+    ⇒ LNTH n (iforest ψ trace) ≠ SOME (p,a)
+Proof
+  rw[] \\ drule not_in_forest_not_in_trace
+  \\ disch_then (qspec_then ‘trace’ assume_tac)
+  \\ gs[every_LNTH]
+  \\ Cases_on ‘LNTH n (iforest ψ trace)’ \\ gs[]
+  \\ first_x_assum drule \\ Cases_on ‘x’ \\ simp[]
+QED
+
+(* If an itree returns in the forest it never does any more actions *)
+Theorem iforest_itree_end:
+  ∀n ψ trace p t.
+    LNTH n (iforest ψ trace) = SOME (p, Res t) ⇒
+      ∀m a. n < m ⇒ LNTH m (iforest ψ trace) ≠ SOME (p,a)
+Proof
+  Induct \\ rw[]
+  >- (gs[Once iforest_def] \\ simp[Once iforest_def]
+      \\ Cases_on ‘next_proc ψ trace’ \\ gs[]
+      \\ Cases_on ‘x’ \\ gs[]
+      \\ drule next_proc_ifores_get_SOME \\ rw[] \\ gs[]
+      \\ Cases_on ‘i’ \\ gs[iforest_act_def,iforest_step_def] \\ rveq
+      \\ Cases_on ‘m’ \\ gs[]
+      \\ irule iforest_not_in_forest
+      \\ simp[iforest_itrees_del])
+  >- (gs[iforest_aux_def,LNTH_LUNFOLD,CaseEq"option",CaseEq"prod"] \\ rveq
+      \\ Cases_on ‘tx’
+      \\ first_x_assum drule
+      \\ cheat)
 QED
 
 val _ = export_theory();
